restructure high-level and low-level specs

specs/experimental/rsapss/high-level/Spec.Bignum.Basic.fst
@@ -9,28 +9,37 @@ open FStar.Math.Lemmas
 
 let bignum bits = n:nat{n < pow2 bits}
 let bn_v #n b = b
-let bn #n a = a
 
-let bn_cast #n m b = bn #m b
+val bn:#n:size_pos -> a:nat{a < pow2 n} -> b:bignum n{bn_v b == a}
+let bn #n b = b
 
-val lemma_bn_add:#n:size_nat -> #m:size_nat{n >= m} -> a:bignum n -> b:bignum m -> Lemma
+let bn_const_1 #n =
+  assert_norm (1 < pow2 n);
+  bn 1
+
+let bn_cast_le #n m b = bn #m b
+let bn_cast_gt #n m b = bn #m b
+
+val lemma_bn_add:#n:size_pos -> #m:size_pos{n >= m} -> a:bignum n -> b:bignum m -> Lemma
   (bn_v a + bn_v b < pow2 (n + 1))
 let lemma_bn_add #n #m a b = admit()
 
 let bn_add #n #m a b =
   lemma_bn_add #n #m a b;
-  bn #(n+1) (a + b)
+  let res = (a + b) % pow2 n in
+  let c = (a + b) / pow2 n in
+  assume (c < pow2 1);
+  (u8 c, bn #n res)
 
-val lemma_bn_mul:#n:size_nat -> #m:size_nat -> a:bignum n -> b:bignum m -> Lemma
+let bn_sub #n #m a b = a - b
+
+val lemma_bn_mul:#n:size_pos -> #m:size_pos -> a:bignum n -> b:bignum m -> Lemma
   (bn_v a * bn_v b < pow2 (n + m))
 let lemma_bn_mul #n #m a b = admit()
- // assert (bn_v a * bn_v b < pow2 n * pow2 m);
 
 let bn_mul #n #m a b =
   lemma_bn_mul #n #m a b;
   bn #(n+m) (a * b)
-
-let bn_sub #n #m a b = a - b
 
 let bn_get_bit #n b i = (b / pow2 i) % 2
 let bn_get_bits #n b i j = (b / pow2 i) % pow2 (j - i)
@@ -46,13 +55,17 @@ let bn_from_u64 c = bn #64 (uint_to_nat c)
 
 let bn_is_less #n x y = x < y
 
-val lemma_bn_lshift_mul_add:#n:size_nat -> #m:size_nat -> x:bignum n -> i:size_nat -> y:bignum 64 -> z:bignum m -> Lemma
+val lemma_bn_lshift_mul_add:#n:size_pos -> #m:size_pos -> x:bignum n -> i:size_nat -> y:bignum 64 -> z:bignum m -> Lemma
   (bn_v x * (pow2 i) * bn_v y + bn_v z < pow2 (m + 1))
 let lemma_bn_lshift_mul_add #n #m x i y z = admit()
 
 let bn_lshift_mul_add #n #m x i y z =
   lemma_bn_lshift_mul_add #n #m x i y z;
-  x * (pow2 i) * y + z
+  let res = x * (pow2 i) * y + z in
+  let r = res % pow2 m in
+  let c = res / pow2 m in
+  assume (c < pow2 1);
+  (u8 c, bn #m r)
 
 let bn_from_bytes_be #bBytes b =
   let res = nat_from_bytes_be b in
